commit

AP/Util/Sigma.lean
@@ -6,3 +6,69 @@ namespace Sigma
 theorem fst_comp_mk_eq_id {α : Type*} {β : α → Type*} {f : (i : α) → β i} :
 ((λ (x : Σ i, β i) => x.fst) ∘ (λ i => ⟨i, f i⟩)) = (λ i => i) := by
   ext x; simp
+
+@[simp]
+def toProd {α β : Type*} (x : Σ (_ : α), β) : α × β :=
+  ⟨x.1, x.2⟩
+
+@[simp]
+theorem prod_to_sigma_comp_sigma_to_prod {α β : Type*} :
+@Sigma.toProd α β ∘ Prod.toSigma = id := by
+  ext:1; simp
+
+@[simp]
+theorem sigma_to_prod_comp_prod_to_sigma {α β : Type*} :
+@Prod.toSigma α β ∘ Sigma.toProd = id := by
+  ext:1; simp
+
+theorem toProd_inj {α β : Type*} {x y : Σ (_ : α), β}
+(h : x.toProd = y.toProd) : x = y := by
+  replace h := congrArg Prod.toSigma h; simp at h; exact h
+
+@[simp]
+theorem toProd_eq_toProd {α β : Type*} {x y : Σ (_ : α), β} :
+x.toProd = y.toProd ↔ x = y :=
+  ⟨toProd_inj, by rintro rfl; rfl⟩
+
+@[simp]
+theorem injective_toProd {α β : Type*} : Function.Injective # @Sigma.toProd α β := by
+  rintro ⟨a, b⟩ ⟨c, d⟩ h; simp at h; simp [h]
+
+end Sigma namespace Option
+
+@[simp]
+theorem map_sigma_toProd_eq_iff {α β : Type*} {ma mb : Option (Σ (_ : α), β)} :
+ma.map Sigma.toProd = mb.map Sigma.toProd ↔ ma = mb := by
+  refine' ⟨λ h => _, by rintro rfl; rfl⟩
+  cases ma <;> cases mb <;> simp at h; rfl
+  nm a b
+  simp
+  ext <;> simp [h]
+
+end Option namespace List
+
+@[simp]
+theorem map_sigma_toProd_eq_iff {α β : Type*} {xs ys : List (Σ (_ : α), β)} :
+xs.map Sigma.toProd = ys.map Sigma.toProd ↔ xs = ys := by
+  refine' ⟨λ h => _, by rintro rfl; rfl⟩
+  rw [map_eq_iff] at h
+  ext
+  nm i x
+  rcases x with ⟨a, b⟩
+  specialize h i
+  simp at h
+  rw [h]
+
+theorem ind_pair_sigma {α β : Type*} {P : List (α × β) → Prop}
+(h : ∀ (xs : List # Σ (_ : α), β), P # xs.map Sigma.toProd)
+(xs : List # α × β) : P xs := by
+  obtain ⟨xs, rfl⟩ : ∃ (ys : List _), ys.map Sigma.toProd = xs :=
+    ⟨xs.map Prod.toSigma, by simp⟩
+  apply h
+
+end List namespace Sigma
+
+@[simp]
+theorem fst_eq_fst_and_eq_iff {α : Type*} {β : α → Type*} {x y : Σ (i : α), β i} :
+x.fst = y.fst ∧ x = y ↔ x = y := by
+  rcases x with ⟨i, x⟩; rcases y with ⟨j, y⟩; simp
