AP.lean
@@ -1,2 +1,2 @@
-import AP.Util.Basic
+import AP.Util.Main
 import Mathlib.Tactic
