AP/Util/Basic.lean
@@ -7,8 +7,8 @@ import AP.Util.Sigma
 import AP.Util.Order
 import AP.Util.Option
 import AP.Util.Fintype
-import AP.Util.HashMap
 import AP.Util.Quotient
 import AP.Util.Multiset
 import AP.Util.SetTheory
+import AP.Util.ExtDHashMap
 import AP.Util.BigOperators
