AP/Util/Data/Main.lean
@@ -1,2 +1,1 @@
-import AP.Util.Data.Set.Main
-import AP.Util.Data.Map.Main
+import AP.Util.Data.Map
