AP/Util/ExtDHashMap.lean
@@ -1,0 +1,196 @@
+import AP.Util.DHashMap
+
+variable {α : Type*} {β : α → Type*} {γ : α → Type*}
+variable [hh₁ : LinearOrder α] [hh₂ : Hashable α]
+variable {mp : Std.ExtDHashMap α β}
+
+namespace Std.ExtDHashMap
+
+@[simp]
+theorem not_mem_empty' {i : α} : i ∉ (∅ : Std.ExtDHashMap α β) :=
+  not_mem_empty
+
+@[simp]
+theorem not_mem_lift_empty {i : α} :
+¬Membership.mem (γ := Std.ExtDHashMap α β) ⟦∅⟧ i :=
+  not_mem_empty
+
+theorem mem_iff_get?_eq_some {i : α} : i ∈ mp ↔ ∃ x, mp.get? i = some x := by
+  rw [←Option.isSome_iff_exists]
+  exact mem_iff_isSome_get?
+
+theorem get?_eq_some_of_mem {i : α} (h : i ∈ mp) : ∃ x, mp.get? i = some x := by
+  rwa [←mem_iff_get?_eq_some]
+
+theorem get?_eq_none_of_not_mem {i : α} (h : i ∉ mp) : mp.get? i = none := by
+  simp [mem_iff_get?_eq_some] at h
+  rwa [Option.eq_none_iff_forall_ne_some]
+
+@[simp]
+theorem get?_eq_none_iff {i} : mp.get? i = none ↔ i ∉ mp := by
+  refine' ⟨_, get?_eq_none_of_not_mem⟩
+  intro h
+  contrapose! h
+  obtain ⟨x, hx⟩ := get?_eq_some_of_mem h
+  simp [hx]
+
+def toList (mp : Std.ExtDHashMap α β) : List (Σ i, β i) :=
+  mp.lift Std.DHashMap.toSortedList # by simp [Std.DHashMap.equiv_def]
+
+@[simp]
+theorem toList_empty : (∅ : Std.ExtDHashMap α β).toList = [] := by
+  change List.mergeSort _ _ = _; simp
+
+@[simp]
+theorem ofList_snoc {xs} {x : Σ i, β i} :
+ofList (xs ++ [x]) = Insert.insert x (ofList xs) := by
+  dsimp
+  unfold Std.ExtDHashMap.ofList Std.ExtDHashMap.insert
+  rw [Std.DHashMap.ofList_snoc]; rfl
+
+@[simp]
+theorem mem_insert' {x : Σ i, β i} {i} :
+i ∈ Insert.insert x mp ↔ i = x.1 ∨ i ∈ mp := by
+  simp; tauto
+
+@[simp]
+theorem mem_ofList' {xs : List (Σ i, β i)} {i} :
+i ∈ ofList xs ↔ ∃ x, ⟨i, x⟩ ∈ xs := by
+  change contains _ _ ↔ _
+  simp only [contains_ofList, List.contains_eq_mem, List.mem_map,
+    Sigma.exists, exists_and_right, exists_eq_right, decide_eq_true_eq]
+
+theorem eq_empty_iff : mp = ∅ ↔ ∀ i, i ∉ mp := by
+  change mp = ⟦∅⟧ ↔ _
+  apply mp.ind
+  intro m
+  rw [Quotient.eq_iff_equiv]
+  change m.Equiv ∅ ↔ _
+  simp
+  exact Std.DHashMap.isEmpty_iff_forall_not_mem
+
+theorem ext_iff' {m₁ m₂ : Std.ExtDHashMap α β} :
+m₁ = m₂ ↔ m₁.out.Equiv m₂.out := by
+  symm
+  induction m₁, m₂ using Quotient.inductionOn₂
+  nm m₁ m₂
+  change ⟦m₁⟧.out ≈ ⟦m₂⟧.out ↔ _
+  rw [Quotient.eq_iff_equiv]
+  simp
+  rfl
+
+theorem ext_iff {m₁ m₂ : Std.ExtDHashMap α β} :
+m₁ = m₂ ↔ ∀ i, m₁.get? i = m₂.get? i := by
+  induction m₁, m₂ using Quotient.inductionOn₂
+  rw [Quotient.eq_iff_equiv]
+  exact Std.DHashMap.equiv_iff_get?
+
+theorem get?_eq_ite_of_unit {m : Std.ExtDHashMap α (λ _ => Unit)} {i} :
+m.get? i = if i ∈ m then some () else none := by
+  split_ifs with h
+  · obtain ⟨x, hx⟩ := get?_eq_some_of_mem h
+    simp [hx]
+  rw [get?_eq_none_of_not_mem h]
+
+theorem ofList_eq_ofList_iff {xs ys : List (Σ i, β i)}
+(hx : (xs.map (·.1)).Nodup) (hy : (ys.map (·.1)).Nodup) :
+ofList xs = ofList ys ↔ xs.Perm ys := by
+  have hx' := hx.of_map _
+  have hy' := hy.of_map _
+  unfold ofList Quotient.mk'
+  rw [Quotient.eq_iff_equiv]
+  change Std.DHashMap.Equiv _ _ ↔ _
+  rw [Std.DHashMap.equiv_iff_toList_perm]
+  rw [List.perm_ext_iff_of_nodup hx' hy']
+  rw [List.perm_ext_iff_of_nodup (by simp) (by simp)]
+  apply forall_congr'
+  rintro ⟨i, x⟩
+  simp
+  generalize h₁ : Std.DHashMap.ofList xs = m₁
+  generalize h₂ : Std.DHashMap.ofList ys = m₂
+  have h₃ : xs.Perm m₁.toList :=
+    by
+      subst h₁
+      exact (Std.DHashMap.toList_ofList_perm hx).symm
+  have h₄ : ys.Perm m₂.toList :=
+    by
+      subst h₂
+      exact (Std.DHashMap.toList_ofList_perm hy).symm
+  rw [h₃.mem_iff, h₄.mem_iff]
+  simp
+
+def range [ha : Fintype α] (f : (i : α) → β i) : Std.ExtDHashMap α β := by
+  rcases ha with ⟨⟨m, hm⟩, ha⟩
+  refine' m.liftWith _ _
+  · intro xs
+    exact ofList # xs.map # λ i => ⟨i, f i⟩
+  clear ha
+  replace hm : m.toList.Nodup := by simpa
+  intro xs ys (hx : m.toList.Perm xs) (hy : m.toList.Perm ys)
+  rw [ofList_eq_ofList_iff]
+  rotate_left
+  · simp; exact hx.nodup hm
+  · simp; exact hy.nodup hm
+  rw [List.map_perm_map_iff]
+  · exact hx.symm.trans hy
+  intro x y h
+  simp at h
+  exact h.1
+
+@[simp]
+theorem mem_range [ha : Fintype α] {f : (i : α) → β i} {i : α} : i ∈ range f := by
+  simp [range]
+  change i ∈ ha.elems.val.toList
+  simp
+
+@[simp]
+theorem nonempty_insert {x} : Insert.insert x mp ≠ ⟦∅⟧ := by
+  apply ne_of_congr (x.1 ∈ ·); simp
+
+@[simp]
+theorem nodup_toList : mp.toList.Nodup := by
+  apply mp.ind; intro mp
+  exact Std.DHashMap.nodup_toSortedList
+
+@[simp]
+theorem sorted_toList : mp.toList.Sorted (·.1 ≤ ·.1) := by
+  apply mp.ind; simp [toList]
+
+@[simp]
+theorem mem_toList {x} : x ∈ mp.toList ↔ mp.get? x.1 = x.2 := by
+  unfold toList get?
+  apply mp.ind
+  intro m
+  rcases x with ⟨i, x⟩
+  simp [Std.DHashMap.toSortedList]
+
+@[simp]
+theorem toList_eq_toList {m₁ m₂ : Std.ExtDHashMap α β} :
+m₁.toList = m₂.toList ↔ m₁ = m₂ := by
+  refine' ⟨λ h => _, λ h => by rw [h]⟩
+  rw [List.eq_iff_of_nodup_and_sorted (·.1 ≤ ·.1)] at h
+  any_goals simp
+  rotate_left
+  · rintro ⟨i, x⟩ ⟨j, y⟩
+    simp
+    intro h₁ h₂ h₃ h₄
+    have h₅ := le_antisymm h₃ h₄
+    subst h₅
+    use rfl
+    simp [h₁] at h₂
+    simpa
+  rw [ext_iff]
+  intro i
+  ext x
+  specialize h ⟨i, x⟩
+  simp at h
+  exact h
+
+@[simp]
+theorem toList_eq_nil_iff : mp.toList = [] ↔ mp = ∅ := by
+  rw [←toList_empty, toList_eq_toList]
+
+def fold {γ : Type*}
+(mp : Std.ExtDHashMap α β) (f : γ → (i : α) → β i → γ) (z : γ)
+(h : ∀ acc i x j y, f (f acc i x) j y = f (f acc j y) i x) : γ :=
+  mp.lift (·.fold f z) # λ _ _ => DHashMap.fold_eq_fold_of_equiv h
